Remove rec_ prefixes
Especially using just [Specification] and [pre]/[post]/[recover] for
fields, since crash specifications do not use those identifiers.

There are still many "r" prefixes (eg, [prog_rok] and [prog_rspec]).

src/Shallow/ProgLang/HoareRecovery.v
@@ -5,44 +5,44 @@ Require Import Hoare.
 
 Set Implicit Arguments.
 
-Record RecQuadruple T R State :=
-  RecSpec {
-      rec_pre: Prop;
-      rec_post: T -> State -> Prop;
-      recover_post: R -> State -> Prop;
+Record Quadruple T R State :=
+  Spec {
+      pre: Prop;
+      post: T -> State -> Prop;
+      recover: R -> State -> Prop;
     }.
 
-Definition RecSpecification A T R State := A -> State -> RecQuadruple T R State.
+Definition Specification A T R State := A -> State -> Quadruple T R State.
 
-Definition prog_rspec `(spec: RecSpecification A T R State) `(p: prog T)
+Definition prog_rspec `(spec: Specification A T R State) `(p: prog T)
            `(rec: prog R)
            `(rf: Refinement State) :=
   forall a w,
     let state := abstraction rf w in
-    rec_pre (spec a state) ->
+    pre (spec a state) ->
     invariant rf w ->
     forall r, rexec p rec w r ->
          match r with
          | RFinished v w' => let state' := abstraction rf w' in
-                            rec_post (spec a state) v state' /\
+                            post (spec a state) v state' /\
                             invariant rf w'
          | Recovered v w' => let state' := abstraction rf w' in
-                            recover_post (spec a state) v state' /\
+                            recover (spec a state) v state' /\
                             invariant rf w'
          end.
 
 Definition rspec_impl
-           `(spec1: RecSpecification A' T R State)
-           `(spec2: RecSpecification A T R State) :=
-  forall a state, rec_pre (spec2 a state) ->
-         exists a', rec_pre (spec1 a' state) /\
-               (forall v state', rec_post (spec1 a' state) v state' ->
-                        rec_post (spec2 a state) v state') /\
-               (forall rv state', recover_post (spec1 a' state) rv state' ->
-                         recover_post (spec2 a state) rv state').
+           `(spec1: Specification A' T R State)
+           `(spec2: Specification A T R State) :=
+  forall a state, pre (spec2 a state) ->
+         exists a', pre (spec1 a' state) /\
+               (forall v state', post (spec1 a' state) v state' ->
+                        post (spec2 a state) v state') /\
+               (forall rv state', recover (spec1 a' state) rv state' ->
+                         recover (spec2 a state) rv state').
 
-Theorem prog_rspec_weaken : forall `(spec1: RecSpecification A T R State)
-                              `(spec2: RecSpecification A' T R State)
+Theorem prog_rspec_weaken : forall `(spec1: Specification A T R State)
+                              `(spec2: Specification A' T R State)
                               `(p: prog T) `(rec: prog R)
                               (rf: Refinement State),
     prog_rspec spec1 p rec rf ->
@@ -81,37 +81,37 @@ Definition prog_rdouble `(pre: RecDoublePre T R State)
                             invariant rf w'
          end.
 
-Definition prog_rok `(spec: RecSpecification A T R State)
+Definition prog_rok `(spec: Specification A T R State)
            `(p: prog T) `(rec: prog R)
            `(rf: Refinement State) :=
   forall T' (rx: T -> prog T'),
     prog_rdouble
       (fun state postcond recpost =>
-         exists a, rec_pre (spec a state) /\
-                   (forall r, prog_rdouble
-                                (fun state' postcond' recpost' =>
-                                   rec_post (spec a state) r state' /\
-                                   postcond' = postcond /\
-                                   recpost' = recpost)
-                                (rx r) rec rf) /\
-                   (forall r state', recover_post (spec a state) r state' ->
-                                     recpost r state')) (Bind p rx) rec rf.
+         exists a, pre (spec a state) /\
+              (forall r, prog_rdouble
+                      (fun state' postcond' recpost' =>
+                         post (spec a state) r state' /\
+                         postcond' = postcond /\
+                         recpost' = recpost)
+                      (rx r) rec rf) /\
+              (forall r state', recover (spec a state) r state' ->
+                       recpost r state')) (Bind p rx) rec rf.
 
 Theorem rdouble_weaken : forall `(p: prog T) `(rec: prog R)
-                                `(rf: Refinement State)
-                                (pre pre': RecDoublePre T R State),
+                           `(rf: Refinement State)
+                           (pre pre': RecDoublePre T R State),
     prog_rdouble pre' p rec rf ->
     (forall state postcond recpost, pre state postcond recpost ->
-                                    pre' state postcond recpost) ->
+                           pre' state postcond recpost) ->
     prog_rdouble pre p rec rf.
 Proof.
   unfold prog_rdouble at 2; intros.
   eapply H; eauto.
 Qed.
 
-Theorem prog_rspec_to_rok : forall `(spec: RecSpecification A T R State)
-                                   `(p: prog T) `(rec: prog R)
-                                   `(rf: Refinement State),
+Theorem prog_rspec_to_rok : forall `(spec: Specification A T R State)
+                              `(p: prog T) `(rec: prog R)
+                              `(rf: Refinement State),
     prog_rspec spec p rec rf ->
     prog_rok spec p rec rf.
 Proof.
@@ -145,8 +145,8 @@ Proof.
 Qed.
 
 Theorem rdouble_exec_equiv : forall `(rf: Refinement State)
-                                    `(pre: RecDoublePre T R State) (p p': prog T)
-                                    (rec: prog R),
+                               `(pre: RecDoublePre T R State) (p p': prog T)
+                               (rec: prog R),
     exec_equiv p p' ->
     prog_rdouble pre p' rec rf ->
     prog_rdouble pre p rec rf.
@@ -188,12 +188,12 @@ Notation "{{ p ; '_' }}" := (prog_rdouble _ (Bind p _) _ _)
 (** * (much simpler) alternative to begin *)
 
 Theorem rdouble_cases : forall `(pre: RecDoublePre T R State)
-                               `(p: prog T) `(rec: prog R)
-                               `(rf: Refinement State),
+                          `(p: prog T) `(rec: prog R)
+                          `(rf: Refinement State),
     (forall state postcond recpost,
         pre state postcond recpost ->
         exists pre', prog_rdouble pre' p rec rf /\
-                     pre' state postcond recpost) ->
+                pre' state postcond recpost) ->
     prog_rdouble pre p rec rf.
 Proof.
   unfold prog_rdouble at 2; intros.
@@ -235,12 +235,12 @@ Proof.
     econstructor; eauto.
 Qed.
 
-Definition prog_rec_loopspec `(spec: RecSpecification A unit unit State)
+Definition prog_loopspec `(spec: Specification A unit unit State)
            `(rec': prog unit) `(rec: prog unit)
            (rf: Refinement State) :=
   forall a w,
     let state := abstraction rf w in
-    rec_pre (spec a state) ->
+    pre (spec a state) ->
     invariant rf w ->
     forall rv rv' w',
       Relation_Operators.clos_refl_trans_1n
@@ -249,31 +249,31 @@ Definition prog_rec_loopspec `(spec: RecSpecification A unit unit State)
       forall rv'' w'',
         exec rec' w' (Finished rv'' w'') ->
         let state'' := abstraction rf w'' in
-        rec_post (spec a state) rv'' state'' /\
+        post (spec a state) rv'' state'' /\
         invariant rf w''.
 
-Definition rec_idempotent `(spec: RecSpecification A T unit State) :=
+Definition idempotent `(spec: Specification A T unit State) :=
   forall a state,
-    rec_pre (spec a state) ->
-    forall v state', recover_post (spec a state) v state' ->
+    pre (spec a state) ->
+    forall v state', recover (spec a state) v state' ->
                      (* idempotency: crash invariant implies precondition to re-run on
                every crash *)
-                     exists a', rec_pre (spec a' state') /\
+                     exists a', pre (spec a' state') /\
                                 (* postcondition transitivity: establishing the postcondition
                    from a crash state is sufficient to establish it with respect
                    to the original initial state (note all with the same ghost
                    state) *)
-                                forall rv state'', rec_post (spec a' state') rv state'' ->
-                                                   rec_post (spec a state) rv state''.
+                                forall rv state'', post (spec a' state') rv state'' ->
+                                                   post (spec a state) rv state''.
 
-Theorem rec_idempotent_loopspec : forall `(rec: prog unit) `(rec': prog unit)
-                                         `(spec: RecSpecification A unit unit State)
-                                         (rf: Refinement State),
+Theorem idempotent_loopspec : forall `(rec: prog unit) `(rec': prog unit)
+                                     `(spec: Specification A unit unit State)
+                                     (rf: Refinement State),
     forall (Hspec: prog_rspec spec rec' rec rf),
-      rec_idempotent spec ->
-      prog_rec_loopspec spec rec' rec rf.
+      idempotent spec ->
+      prog_loopspec spec rec' rec rf.
 Proof.
-  unfold prog_rec_loopspec; intros.
+  unfold prog_loopspec; intros.
   apply clos_refl_trans_1n_unit_tuple in H2.
   repeat match goal with
          | [ u: unit |- _ ] => destruct u
@@ -288,24 +288,24 @@ Proof.
     specialize (IHclos_refl_trans_1n a'); intuition eauto.
 Qed.
 
-Theorem compose_recovery : forall `(spec: RecSpecification A'' T unit State)
-                                  `(rspec: RecSpecification A' unit unit State)
-                                  `(spec': RecSpecification A T unit State)
+Theorem compose_recovery : forall `(spec: Specification A'' T unit State)
+                                  `(rspec: Specification A' unit unit State)
+                                  `(spec': Specification A T unit State)
                                   `(p: prog T) `(rec: prog unit) `(rec': prog unit)
                                   `(rf: Refinement State),
     forall (Hspec: prog_rspec spec p rec rf)
-           (Hrspec: prog_rec_loopspec rspec rec' rec rf)
+           (Hrspec: prog_loopspec rspec rec' rec rf)
            (Hspec_spec':
-              forall (a:A) state, rec_pre (spec' a state) ->
+              forall (a:A) state, pre (spec' a state) ->
                                   exists (a'':A''),
-                                    rec_pre (spec a'' state) /\
-                                    (forall v state', rec_post (spec a'' state) v state' ->
-                                                      rec_post (spec' a state) v state') /\
-                                    (forall v state', recover_post (spec a'' state) v state' ->
-                                                      exists a', rec_pre (rspec a' state') /\
+                                    pre (spec a'' state) /\
+                                    (forall v state', post (spec a'' state) v state' ->
+                                                      post (spec' a state) v state') /\
+                                    (forall v state', recover (spec a'' state) v state' ->
+                                                      exists a', pre (rspec a' state') /\
                                                                  forall v' state'',
-                                                                   rec_post (rspec a' state') v' state'' ->
-                                                                   recover_post (spec' a state) v' state'')),
+                                                                   post (rspec a' state') v' state'' ->
+                                                                   recover (spec' a state) v' state'')),
       prog_rspec spec' p (_ <- rec; rec') rf.
 Proof.
   intros.
@@ -331,8 +331,8 @@ Proof.
     | [ Hexec: rexec p _ _ _ |- _ ] =>
       eapply Hspec in Hexec
     end; simpl in *; safe_intuition eauto.
-    (* H5: recover_post -> exists a' *)
-    (* H1: recover_post *)
+    (* H5: recover -> exists a' *)
+    (* H1: recover *)
     eapply H5 in H1; repeat deex.
     match goal with
     | [ Hexec: exec rec' _ _ |- _ ] =>
@@ -341,24 +341,24 @@ Proof.
 Qed.
 
 Theorem rspec_refinement_compose :
-  forall `(spec: RecSpecification A T R State2)
-    `(p: prog T) `(rec: prog R)
-    `(rf2: LRefinement State1 State2)
-    `(rf1: Refinement State1),
+  forall `(spec: Specification A T R State2)
+         `(p: prog T) `(rec: prog R)
+         `(rf2: LRefinement State1 State2)
+         `(rf1: Refinement State1),
     prog_rspec
       (fun (a:A) state =>
          let state2 := abstraction rf2 state in
-         {| rec_pre := rec_pre (spec a state2) /\
-                       invariant rf2 state;
-            rec_post :=
+         {| pre := pre (spec a state2) /\
+                   invariant rf2 state;
+            post :=
               fun v state' =>
                 let state2' := abstraction rf2 state' in
-                rec_post (spec a state2) v state2' /\
+                post (spec a state2) v state2' /\
                 invariant rf2 state';
-            recover_post :=
+            recover :=
               fun v state' =>
                 let state2' := abstraction rf2 state' in
-                recover_post (spec a state2) v state2' /\
+                recover (spec a state2) v state2' /\
                 invariant rf2 state'; |}) p rec rf1 ->
     prog_rspec spec p rec (refinement_compose rf1 rf2).
 Proof.
@@ -379,22 +379,22 @@ Definition rec_noop `(rec: prog R) `(rf: Refinement State) :=
   forall T (v:T),
     prog_rspec
       (fun (_:unit) state =>
-         {| rec_pre := True;
-            rec_post := fun r state' => r = v /\
-                                 state' = state;
-            recover_post := fun _ state' => state' = state; |}) (Ret v) rec rf.
+         {| pre := True;
+            post := fun r state' => r = v /\
+                             state' = state;
+            recover := fun _ state' => state' = state; |}) (Ret v) rec rf.
 
 Hint Resolve tt.
 
-Theorem prog_rok_to_rspec : forall `(spec: RecSpecification A T R State)
+Theorem prog_rok_to_rspec : forall `(spec: Specification A T R State)
                               `(p: prog T) `(rec: prog R)
                               `(rf: Refinement State),
     prog_rok spec p rec rf ->
     rec_noop rec rf ->
-    (forall a state, rec_pre (spec a state) ->
+    (forall a state, pre (spec a state) ->
             forall v state',
-              rec_post (spec a state) v state' ->
-              forall rv, recover_post (spec a state) rv state') ->
+              post (spec a state) v state' ->
+              forall rv, recover (spec a state) rv state') ->
     prog_rspec spec p rec rf.
 Proof.
   unfold prog_rok, prog_rdouble, prog_rspec; intros.
@@ -416,12 +416,12 @@ Qed.
 (* for recovery proofs about pure programs *)
 
 Theorem ret_prog_rok : forall `(rf: Refinement State)
-                         `(spec: RecSpecification A T R State)
+                         `(spec: Specification A T R State)
                          (v:T) (rec: prog R),
     rec_noop rec rf ->
-    (forall a state, rec_pre (spec a state) ->
-            rec_post (spec a state) v state /\
-            forall r, recover_post (spec a state) r state) ->
+    (forall a state, pre (spec a state) ->
+            post (spec a state) v state /\
+            forall r, recover (spec a state) r state) ->
     prog_rok spec (Ret v) rec rf.
 Proof.
   intros.
@@ -442,11 +442,11 @@ Theorem rec_noop_compose : forall `(rec: prog unit) `(rec2: prog unit)
     rec_noop rec rf1 ->
     prog_rspec
       (fun (_:unit) state =>
-         {| rec_pre := invariant rf2 state;
-            rec_post :=
+         {| pre := invariant rf2 state;
+            post :=
               fun _ state' => invariant rf2 state' /\
                        abstraction rf2 state' = abstraction rf2 state;
-            recover_post :=
+            recover :=
               fun _ state' => invariant rf2 state' /\
                        abstraction rf2 state' = abstraction rf2 state;
          |}) rec2 rec rf1 ->
@@ -455,8 +455,8 @@ Proof.
   unfold rec_noop; intros.
   eapply rspec_refinement_compose; simpl.
   eapply compose_recovery; eauto.
-  eapply rec_idempotent_loopspec; eauto.
-  unfold rec_idempotent; simpl; intuition eauto.
+  eapply idempotent_loopspec; eauto.
+  unfold idempotent; simpl; intuition eauto.
   descend; intuition (eauto; congruence).
   simpl; intuition.
   descend; intuition (subst; eauto).
